

**Université Paris 1 Panthéon Sorbonne**

**UFR27 - MMMEF - Yiel Curve Models**



# **Project Explicit Finite Differencies**

**Lola Chardigny, Abderrahmane Louirem**

January 2025

# Contents

<b>1</b>	<b>Black-Scholes Equation</b>	<b>2</b>
1.1	The equation . . . . .	2
1.2	Change of variable . . . . .	2
1.3	Euler scheme and discretization . . . . .	3
1.4	Boundary conditions . . . . .	4
<b>2</b>	<b>Implementation</b>	<b>5</b>

# 1 Black-Scholes Equation

## 1.1 The equation

In a B&S framework:

$$dX(t) = X(t)r dt + X(t)\sigma dW(t) \quad (1)$$

$$X(0) = X_0$$

Infinitesimal linear generator

$$f(t, x) \rightarrow \mathcal{L}^X f(t, x) = \frac{\partial f}{\partial t} + rx \frac{\partial f}{\partial x} + \frac{1}{2} \sigma^2 x^2 \frac{\partial^2 f}{\partial x^2}$$

Initial PDE :

$$P(L, G) = \begin{cases} Lf = 0 \\ f(T, x) = G(x) \end{cases}$$

where  $Lf \equiv \mathcal{L}^X f - rf$ .

## 1.2 Change of variable

Let  $Y(t) = \ln(X(t))$ , the logarithm of the price of the underlying, and let  $h(t, Y(t)) \equiv f(t, \ln(X(t)))$ , the price of the option expressed as a function of the logarithm of the price. **Show that  $h$  is the solution of:**

$$\begin{cases} \frac{\partial h}{\partial t} + \left(r - \frac{1}{2}\sigma^2\right) \frac{\partial h}{\partial x} + \frac{1}{2}\sigma^2 \frac{\partial^2 h}{\partial x^2} = rh \\ h(T, x) = G(e^x) \end{cases}$$

We rewrite our three partial differentials (and we recall that  $(U + V)' = U'V + UV'$ ):

$$\begin{aligned} \frac{\partial f(t, \ln(X))}{\partial t} &= \frac{\partial h(t, Y)}{\partial t} \\ \frac{\partial f(t, \ln(X))}{\partial x} &= \frac{1}{X} \frac{\partial f(t, \ln(X))}{\partial x} = \frac{1}{X} \cdot \frac{\partial h(t, Y)}{\partial x} \\ \frac{\partial^2 f(t, \ln(X))}{\partial x^2} &= -\frac{1}{X^2} \frac{\partial f(t, \ln(X))}{\partial x} + \frac{1}{X^2} \frac{\partial^2 f(t, \ln(X))}{\partial x^2} = -\frac{1}{X^2} \frac{\partial h(t, Y)}{\partial x} + \frac{1}{X^2} \frac{\partial^2 h(t, Y)}{\partial x^2} \end{aligned}$$

Initially, we have this equation  $\frac{\partial f}{\partial t} + rx \frac{\partial f}{\partial x} + \frac{1}{2} \sigma^2 x^2 \frac{\partial^2 f}{\partial x^2} - rf = 0$  and  $h(t, Y(t)) = f(t, \ln(X(t)))$  where  $Y(t) = \ln(X(t)) \iff X(t) = e^{Y(t)}$   
So we can replace the partial derivatives by the new one inside the initial equation:

$$\begin{aligned}
&\Rightarrow \frac{\partial h}{\partial t} + r \frac{\partial h}{\partial x} + \frac{1}{2} \sigma^2 x^2 \left( -\frac{1}{x^2} \frac{\partial h}{\partial x} + \frac{1}{x^2} \frac{\partial^2 h}{\partial x^2} \right) - rh = 0, \\
&\Rightarrow \frac{\partial h}{\partial t} + r \frac{\partial h}{\partial x} + \left( \frac{1}{2} \sigma^2 \frac{\partial^2 h}{\partial x^2} - \frac{1}{2} \sigma^2 \frac{\partial h}{\partial x} \right) - rh = 0, \\
&\Rightarrow \frac{\partial h}{\partial t} + \frac{\partial h}{\partial x} \left( r - \frac{1}{2} \sigma^2 \right) + \frac{1}{2} \sigma^2 \frac{\partial^2 h}{\partial x^2} = rh.
\end{aligned}$$

with  $h(T, x) = G(e^x)$

### 1.3 Euler scheme and discretization

The domain of  $f$  is  $[0, T] \times \mathbb{R}^+$

We consider the interval  $[X_{\min}, X_{\max}]$

For discretization :

- Time:  $\tau = \{t_0 = 0, \dots, t_j = j\delta t, \dots, t_{\text{ntime}} = T\}$  with  $\delta t = T/\text{ntime}$ ,
- Space:  $\chi = \{x_0 = X_{\min}, \dots, x_i = x_{\min} + i\delta x, \dots, x_{\text{nspace}} = X_{\max}\}$  with  $\delta x = \frac{X_{\max} - X_{\min}}{\text{nspace}}$ . We denote  $\hat{\chi}$  the set  $\chi$  without its boundaries  $X_{\min}$  and  $X_{\max}$ .

Define  $h(j, i) = h(t_j, x_i)$ . **Approximate the partial derivatives using  $h(j, i)$  values on  $\hat{\chi}$  and show that**

$$\begin{aligned}
h(j, i) = h(j+1, i) + \delta t &\left[ \frac{1}{2} \sigma^2 \frac{h(j+1, i+1) - 2h(j+1, i) + h(j+1, i-1)}{(\delta x)^2} \right. \\
&\left. + \left( r - \frac{1}{2} \sigma^2 \right) \frac{h(j+1, i+1) - h(j+1, i-1)}{2\delta x} - rh(j+1, i) \right] + o(1).
\end{aligned}$$

Let us consider  $h(j, i) = h(t_j, x_i) = h_i^j$ .

We compute the three partial derivatives for the FDM:

for the **forward method** we use :

$$\begin{aligned}
\frac{\partial h_i^j}{\partial t} &\approx \frac{h_i^{j+1} - h_i^j}{\delta t} + o(\delta t) \\
\frac{\partial h_i^j}{\partial x} &\approx \frac{h_{i+1}^j - h_{i-1}^j}{2\delta x} + o((\delta x)^2) \\
\frac{\partial^2 h_i^j}{\partial x^2} &\approx \frac{h_{i+1}^j - 2h_i^j + h_{i-1}^j}{(\delta x)^2} + o((\delta x)^2)
\end{aligned}$$

but we prefer the **backward method**, so we use :

$$\begin{aligned}\frac{\partial h_i^j}{\partial t} &\approx \frac{h_i^{j+1} - h_i^j}{\delta t} + o(\delta t) \\ \frac{\partial h_i^j}{\partial x} &\approx \frac{h_{i+1}^{j+1} - h_{i-1}^{j+1}}{2\delta x} + o((\delta x)^2) \\ \frac{\partial^2 h_i^j}{\partial x^2} &\approx \frac{h_{i+1}^{j+1} - 2h_i^{j+1} + h_{i-1}^{j+1}}{(\delta x)^2} + o((\delta x)^2)\end{aligned}$$

The PDE is the following:

$$\frac{\partial h}{\partial t} + \left(r - \frac{1}{2}\sigma^2\right) \frac{\partial h}{\partial x} + \frac{1}{2}\sigma^2 \frac{\partial^2 h}{\partial x^2} - rh = 0$$

and by replacing the partial differentials, we get:

$$\frac{h_i^{j+1} - h_i^j}{\delta t} + \left(r - \frac{1}{2}\sigma^2\right) \frac{h_{i+1}^{j+1} - h_{i-1}^{j+1}}{2\delta x} + \frac{1}{2}\sigma^2 \frac{h_{i+1}^{j+1} - 2h_i^{j+1} + h_{i-1}^{j+1}}{(\delta x)^2} - rh_i^j + o(\delta t) = 0$$

$$\iff h_i^{j+1} - h_i^j + \delta t \left[ \left(r - \frac{1}{2}\sigma^2\right) \frac{h_{i+1}^{j+1} - h_{i-1}^{j+1}}{2\delta x} + \frac{1}{2}\sigma^2 \frac{h_{i+1}^{j+1} - 2h_i^{j+1} + h_{i-1}^{j+1}}{(\delta x)^2} - rh_i^j \right] + o(1) = 0$$

We can take the derivative of  $h$  in  $j$  or  $j + 1$ , it does not matter.

$$\iff h_i^j = h_i^{j+1} + \delta t \left[ \frac{1}{2}\sigma^2 \frac{h_{i+1}^{j+1} - 2h_i^{j+1} + h_{i-1}^{j+1}}{(\delta x)^2} + \left(r - \frac{1}{2}\sigma^2\right) \frac{h_{i+1}^{j+1} - h_{i-1}^{j+1}}{2\delta x} - rh_i^{j+1} \right] + o(1)$$

## 1.4 Boundary conditions

The previous equation holds for  $\mathbf{i} = 1, \dots, \mathbf{n\_space}$  as  $\mathbf{h}_{-1}^j$  and  $\mathbf{h}_{\mathbf{n\_space}+1}^j$  are not defined. Then we have  $\mathbf{n\_space} - 1$  equations for  $\mathbf{n\_space} + 1$  unknowns.

The 2 remaining equations come from the 2 boundary conditions  $\mathbf{i} = \mathbf{0}$  ( $\mathbf{x}_i = \mathbf{x}_0$ ) and  $\mathbf{i} = \mathbf{n\_space}$  ( $\mathbf{x}_i = \mathbf{x}_{\mathbf{n\_space}}$ ).

We assume that  $\forall j : \frac{\partial^2 h}{\partial x^2}(t_j, x_0) = \frac{\partial^2 h}{\partial x^2}(t_j, x_{\mathbf{n\_space}}) = 0$

Use noncentered estimators of the first derivative and **write the discretisation equations for  $i = 0$  and  $i = \mathbf{n\_space}$ .**

$$\frac{\partial^2 h}{\partial x^2}(t_j, x_0) = \frac{\partial^2 h}{\partial x^2}(t_j, x_{\mathbf{n\_space}}) = 0 \iff \frac{\partial h_0^j}{\partial x} = \frac{h_{\mathbf{n\_space}}^j}{\partial x^2} = 0$$

For  $i = 0$  ( $x_i = x_0 = X_{\min}$ ):

$$\text{we get } h_0^j = h_0^{j+1} + \delta t \left( r - \frac{1}{2}\sigma^2 \right) \frac{h_1^{j+1} - h_0^{j+1}}{\delta x} - rh_0^{j+1}$$

For  $i = nspace$  ( $x_i = x_{nspace} = X_{\max}$ ):

$$\text{we get } h_{nspace}^j = h_{nspace}^{j+1} + \delta t \left( r - \frac{1}{2} \sigma^2 \right) \frac{h_{nspace}^{j+1} - h_{nspace-1}^{j+1}}{\delta x} - r h_{nspace}^{j+1}$$

## 2 Implementation

Python.